---
layout: post
title: "Expanding $e^x$ without calculus"
data: 2024-01-04 09:12:00 
categories: Euler's Number
---

2025 ðŸŽ†

A quick proof of the taylor series of $e^x$ without using derivatives.

$$
e^x = \lim_{n \to \infty} \left(1+\frac{x}{n}\right)^{n} \\
\ \\
\text{Using binomial expansion:} \\
\ \\
e^x = \lim_{n \to \infty} \sum_{k=0}^{n} \binom{n}{k} \cdot \frac{x^k}{n^k}  \\
\ \\
= \lim_{n \to \infty} \sum_{k=0}^{n} \frac{n(n-1) \ldots (n-k+1)}{k!} \cdot \frac{x^k}{n^k} \\
\ \\
= \sum_{k=0}^{n} \frac{x^k}{k!} \cdot \underbrace{\lim_{n \to \infty} \frac{n(n-1) \ldots (n-k+1)}{n^k}}_{=1} \\
\ \\
= \sum_{k=0}^{n} \frac{x^k}{k!}
$$
